force env to be empty => much easier proofs

Simu/Cor2.v
@@ -75,7 +75,7 @@ Section PRESERVATION.
 
   Inductive well_formed_exp (c: class): exp -> Prop :=
   | wf_var: forall x ty,
-      In (x, ty) c.(c_vars) ->
+      In (x, ty) (class_vars c) ->
       x <> self_id ->
       well_formed_exp c (Var x ty)
   | wf_state: forall x ty,
@@ -86,7 +86,7 @@ Section PRESERVATION.
 
   Inductive well_formed_stmt (c: class) (S: state): stmt -> Prop :=
   | wf_assign: forall x e (* v *),
-      In (x, typeof e) c.(c_vars) ->
+      In (x, typeof e) (class_vars c) ->
       x <> self_id ->
       well_formed_exp c e ->
       (* exp_eval S e v -> *)
@@ -111,8 +111,8 @@ Section PRESERVATION.
       stmt_eval prog S s1 S' ->
       well_formed_stmt c S' s2 ->
       well_formed_stmt c S (Comp s1 s2)
-  | wf_step: forall y ty c' prog' clsid o es vs me (*me' rv *),
-      In (y, ty) c.(c_vars) ->
+  | wf_step: forall y ty c' prog' clsid o es vs me me' rv,
+      In (y, ty) (class_vars c) ->
       y <> self_id ->
       In {| obj_inst := o; obj_class := clsid |} c.(c_objs) ->
       find_class clsid prog = Some (c', prog') ->
@@ -124,8 +124,9 @@ Section PRESERVATION.
       (* well_formed_stmt c' S c'.(c_step) -> *)
       find_inst o S me ->
       well_formed_stmt c' (me, adds (Nelist.map_fst c'.(c_input)) vs v_empty) c'.(c_step) ->
-      (* stmt_step_eval prog me clsid vs me' rv -> *)
-      (* valid_val rv ty -> *)
+      stmt_step_eval prog me clsid vs me' rv ->
+      valid_val rv ty ->
+      ty <> Ctypes.Tvoid ->
       (* rv = Values.Val.load_result (chunk_of_typ ty) rv -> *)
       well_formed_stmt c S (Step_ap y ty clsid o es)
   | wf_skip: 
@@ -136,7 +137,7 @@ Section PRESERVATION.
   Definition compat_vars (c: class) (S: state) (le: Clight.temp_env): Prop :=
     forall x t v,
       In c prog ->
-      In (x, t) c.(c_vars) ->
+      In (x, t) (class_vars c)->
       find_var x S v ->
       Maps.PTree.get x le = Some v.
 
@@ -304,36 +305,38 @@ Section PRESERVATION.
                        (Memdata.size_chunk (chunk_of_typ t)))
          (Int.unsigned (Int.add ofs (Int.repr delta')))).
 
-  Definition match_step (e: Clight.env) :=
+  Definition match_step (* (e: Clight.env) *) :=
     forall c,
       In c prog ->
       exists loc_f f,
         Globalenvs.Genv.find_symbol tge.(Clight.genv_genv) (step_id c.(c_name)) = Some loc_f
-        /\ Maps.PTree.get (step_id c.(c_name)) e = None
+        (* /\ Maps.PTree.get (step_id c.(c_name)) e = None *)
         /\ Globalenvs.Genv.find_funct_ptr tge.(Clight.genv_genv) loc_f = Some (Ctypes.Internal f)
         /\ Clight.type_of_fundef (Ctypes.Internal f) =
           Ctypes.Tfunction (Ctypes.Tcons (type_of_inst_p c.(c_name))
                                          (list_type_to_typelist (map snd (nelist2list c.(c_input)))))
                            (snd c.(c_output)) AST.cc_default
-        /\ Coqlib.list_norepet (Clight.var_names (Clight.fn_vars f))
+        /\ f.(Clight.fn_vars) = []
+        (* /\ Coqlib.list_norepet (Clight.var_names (Clight.fn_vars f)) *)
         /\ Coqlib.list_norepet (Clight.var_names (Clight.fn_params f))
         /\ Coqlib.list_disjoint (Clight.var_names (Clight.fn_params f)) (Clight.var_names (Clight.fn_temps f))
-        /\ Clight.fn_body f = translate_stmt c.(c_name) c.(c_step)
+        /\ Clight.fn_body f = Clight.Ssequence (translate_stmt c.(c_name) c.(c_step))
+                                              (Clight.Sreturn (Some (Clight.Etempvar (fst c.(c_output)) (snd c.(c_output)))))
         (* /\ length f.(Clight.fn_params) = 1 + Nelist.length c.(c_input) *)
         /\ f.(Clight.fn_params) = (self_id, type_of_inst_p c.(c_name)) :: Nelist.nelist2list c.(c_input)
         /\ Forall (fun x => Ctypes.access_mode (snd x) = Ctypes.By_value (chunk_of_typ (snd x)))
-                 (f.(Clight.fn_params) ++ f.(Clight.fn_vars)).
+                 (f.(Clight.fn_params) (* ++ f.(Clight.fn_vars) *)).
   
-  Definition c_state := (Clight.env * Clight.temp_env * Memory.Mem.mem)%type.
+  Definition c_state := ((* Clight.env * *) Clight.temp_env * Memory.Mem.mem)%type.
    
   Inductive match_states_bigbig (c: class) (S: state): c_state -> Prop :=
-    intro_state_bigbig: forall e le m,
+    intro_state_bigbig: forall (* e *) le m,
       (* state correspondance *)
       compat_vars c S le ->
       compat_self c S le m ->
 
       (* function *)
-      match_step e ->
+      match_step (* e *) ->
       
       (* Clight side separation *)
       fields_sep m ->
@@ -341,16 +344,16 @@ Section PRESERVATION.
       (* Minimp side separation *)
       nodup_mems c ->
       
-      match_states_bigbig c S (e, le, m).
+      match_states_bigbig c S ((* e, *) le, m).
 
   Hint Constructors match_states_bigbig.
   
   Lemma compat_assign_pres:
-    forall c S e le m x v,
+    forall c S (* e *) le m x v,
       In c prog ->
-      match_states_bigbig c S (e, le, m) ->
+      match_states_bigbig c S ((* e, *) le, m) ->
       x <> self_id ->
-      match_states_bigbig c (update_var x S v) (e, Maps.PTree.set x v le, m).
+      match_states_bigbig c (update_var x S v) ((* e,  *)Maps.PTree.set x v le, m).
   Proof.
     introv ? MS ?.
     inverts MS as Hvars Hself.
@@ -386,9 +389,9 @@ Section PRESERVATION.
   Qed.
   
   Lemma compat_stassign_pres:
-    forall c S e le m x t v co loc_struct ofs delta,
+    forall c S (* e *) le m x t v co loc_struct ofs delta,
       In c prog ->
-      match_states_bigbig c S (e, le, m) ->
+      match_states_bigbig c S ((* e, *) le, m) ->
       Ctypes.field_offset tge.(Clight.genv_cenv) x (Ctypes.co_members co) = Errors.OK delta ->
       Maps.PTree.get c.(c_name) (Clight.genv_cenv tge) = Some co ->
       Maps.PTree.get self_id le = Some (Values.Vptr loc_struct ofs) ->
@@ -398,7 +401,7 @@ Section PRESERVATION.
      Memory.Mem.valid_access m (chunk_of_typ t) loc_struct (Int.unsigned (Int.add ofs (Int.repr delta))) Memtype.Writable ->
       exists m',
         Memory.Mem.store (chunk_of_typ t) m loc_struct (Int.unsigned (Int.add ofs (Int.repr delta))) v = Some m'
-        /\ match_states_bigbig c (update_field x S v) (e, le, m').
+        /\ match_states_bigbig c (update_field x S v) ((* e, *) le, m').
   Proof.
     intros ** ? MS Hoffset Hget_co Hget_self Hin Hloadres ? ? .
     inverts MS as Hvars Hself ? Hfields_sep Hnodupmems. 
@@ -432,19 +435,19 @@ Section PRESERVATION.
         rewrite <-Hload; apply* Memory.Mem.load_store_other.          
   Qed.
   
-  Remark alloc_exists:
-    forall vars e m,
-      exists e' m',
-        Clight.alloc_variables tge e m vars e' m'.
-  Proof.
-    induction vars as [|(x, ty)].
-    - do 3 econstructor. 
-    - intros.
-      destruct (Memory.Mem.alloc m 0 (Ctypes.sizeof (Clight.genv_cenv tge) ty)) eqn: Eq.
-      specialize (IHvars (Maps.PTree.set x (b, ty) e) m0).
-      destruct* IHvars as (? & ? & ?).
-      do 3 econstructor; eauto.
-  Qed.
+  (* Remark alloc_exists: *)
+  (*   forall vars e m, *)
+  (*     exists e' m', *)
+  (*       Clight.alloc_variables tge e m vars e' m'. *)
+  (* Proof. *)
+  (*   induction vars as [|(x, ty)]. *)
+  (*   - do 3 econstructor.  *)
+  (*   - intros. *)
+  (*     destruct (Memory.Mem.alloc m 0 (Ctypes.sizeof (Clight.genv_cenv tge) ty)) eqn: Eq. *)
+  (*     specialize (IHvars (Maps.PTree.set x (b, ty) e) m0). *)
+  (*     destruct* IHvars as (? & ? & ?). *)
+  (*     do 3 econstructor; eauto. *)
+  (* Qed. *)
 
   Remark bind_parameter_temps_exists:
     forall xs vs le,
@@ -460,9 +463,9 @@ Section PRESERVATION.
   Qed.
 
   Remark find_var_aux:
-    forall x x' me v v' vs vptr le le',
+    forall x x' y me v v' vs vptr le le',
       find_var x (me, adds (nebase x') (necons v' vs) v_empty) v ->
-      Some (Maps.PTree.set x' v' (Maps.PTree.set self_id vptr le)) = Some le' ->
+      Some (Maps.PTree.set x' v' (Maps.PTree.set y vptr le)) = Some le' ->
       Maps.PTree.get x le' = Some v.
   Proof.
     introv Find Bind.
@@ -476,53 +479,130 @@ Section PRESERVATION.
       apply Maps.PTree.gss.
     - rewrite PM.gso, PM.gempty in Find; auto. discriminate.
   Qed.
+
+  Theorem not_in_cons {A} (x a : A) (l : list A):
+    ~ In x (a::l) <-> x <> a /\ ~ In x l.
+  Proof.
+    split.
+    - intro Notin.
+      split.
+      + intro Eq.
+        apply Notin.
+        rewrite Eq.
+        apply in_eq.
+      + intro In.
+        apply Notin.
+        apply in_cons; auto.
+    - intros [Neq Notin] In.
+      apply in_inv in In.
+      destruct In.
+      + apply Neq; auto.
+      + apply Notin; auto.
+  Qed.
+
+  Theorem set_comm:
+    forall x x' (v v': val) m,
+      x <> x' ->
+      Maps.PTree.set x v (Maps.PTree.set x' v' m) = Maps.PTree.set x' v' (Maps.PTree.set x v m).
+  Admitted.
   
-  Remark bind_parameters_temp_implies:
-    forall c x me vs v vptr le le',
-      find_var x (me, adds (map_fst (c_input c)) vs v_empty) v ->
-      Clight.bind_parameter_temps ((self_id, type_of_inst_p c.(c_name)) :: nelist2list c.(c_input))
+  Remark bind_parameters_temps_cons:
+    forall x t xs v vs le le',
+      Coqlib.list_norepet (Clight.var_names ((x, t) :: xs)) ->
+      Clight.bind_parameter_temps ((x, t) :: xs) (v :: vs) le = Some le' ->
+      Maps.PTree.get x le' = Some v.
+  Proof.
+    induction xs as [|[x' t']]; destruct vs; introv Norep Bind; inverts Bind as Bind.
+    - apply Maps.PTree.gss.
+    - inverts Norep as Notin Norep.
+      apply not_in_cons in Notin.
+      apply* IHxs.
+      + constructor.
+        * apply Notin.
+        * inverts Norep as Notin' Norep.
+          apply Norep.
+      + simpl.
+        rewrite* set_comm in Bind.
+  Qed.
+
+  Remark bind_parameters_temps_implies:
+    forall xs x me vs v vptr xptr le le',
+      Coqlib.list_norepet (Clight.var_names (nelist2list xs)) ->
+      find_var x (me, adds (map_fst xs) vs v_empty) v ->
+      Clight.bind_parameter_temps (xptr :: nelist2list xs)
                                   (vptr :: nelist2list vs) le = Some le' ->
       Maps.PTree.get x le' = Some v.
   Proof.
-    admit.
+    induction xs; destruct vs, xptr; introv Norep Find Bind.
+    - destruct e; inverts Bind as Bind; simpl in Find.
+      apply* find_var_aux.
+    - destruct e; inverts Bind as Bind; simpl in Find.
+      destruct (nelist2list vs).
+      + apply* find_var_aux.
+      + discriminate.
+    - destruct e; inverts Bind as Bind; simpl in Find.
+      destruct (nelist2list xs) eqn: E.
+      + contradict E.
+        apply nelist2list_non_empty.
+      + inverts Bind.
+        destruct p.
+        discriminate.
+    - unfold Clight.bind_parameter_temps in Bind.
+      fold Clight.bind_parameter_temps in Bind.
+      do 2 rewrite nelist2list_cons in Bind.
+      destruct e; simpl in Find.
+      unfold adds, find_var in Find; simpl in Find.
+      destruct (AST.ident_eq x i0).
+      + subst i0.
+        apply find_add in Find.
+        subst e0.
+        apply* bind_parameters_temps_cons.
+      + apply* IHxs.
+        * inverts Norep; auto.
+        * unfold find_var, adds; simpl.
+          rewrite* PM.gso in Find.
+
+          Grab Existential Variables.
+          exact me.
+          exact (nebase e0).
   Qed.
   
   Lemma compat_funcall_pres:
-    forall c m S' S o f me vargs vptr vs,
+    forall c (* e le *) m S o f me vargs loc_struct ofs vs,
       Datatypes.length (Clight.fn_params f) = Datatypes.length vargs ->
       Clight.fn_params f = (self_id, type_of_inst_p c.(c_name)) :: nelist2list c.(c_input) ->
-      match_states_bigbig c S S' ->
-      vargs = vptr :: (Nelist.nelist2list vs) ->
+      Coqlib.list_norepet (Clight.var_names (Clight.fn_params f)) ->
+      (* match_states_bigbig c S (e, le, m) -> *)
+      vargs = (Values.Vptr loc_struct ofs) :: (Nelist.nelist2list vs) ->
       find_inst o S me ->
-      exists m_fun e_fun le_fun,
-        Clight.alloc_variables tge Clight.empty_env m f.(Clight.fn_vars) e_fun m_fun 
-        /\ Clight.bind_parameter_temps f.(Clight.fn_params) vargs (Clight.create_undef_temps f.(Clight.fn_temps))
+      exists (* m_fun e_fun *) le_fun,
+        (* Clight.alloc_variables tge Clight.empty_env m f.(Clight.fn_vars) e_fun m_fun  *)
+        Clight.bind_parameter_temps f.(Clight.fn_params) vargs (Clight.create_undef_temps f.(Clight.fn_temps))
           = Some le_fun
-        /\ match_states_bigbig c (me, adds (map_fst c.(c_input)) vs v_empty) (e_fun, le_fun, m_fun).
+        /\ match_states_bigbig c (me, adds (map_fst c.(c_input)) vs v_empty) ((* e_fun, *) le_fun, m).
   Proof.
-    introv Hlengths Hparams MS ? ?.
-    forwards (e_fun & m_fun & ?): (alloc_exists f.(Clight.fn_vars) Clight.empty_env m).
+    introv Hlengths Hparams Norep (* MS *) ? ?.
+    (* forwards (e_fun & m_fun & ?): (alloc_exists f.(Clight.fn_vars) Clight.empty_env m). *)
     forwards (le_fun & Bind): bind_parameter_temps_exists Hlengths.
-    do 3 econstructor; splits*.
-    inverts MS.
+    econstructor; split*.
+    (* inverts MS. *)
     constructor*.
     - unfold compat_vars.
       intros x' t' v' ? Hin Hfind.
       subst vargs.
-      rewrite Hparams in Bind.
-      apply* bind_parameters_temp_implies.
-
+      rewrite Hparams in Bind, Norep.
+      inverts Norep.
+      apply* bind_parameters_temps_implies.     
+      
     - unfold compat_self.
-      intros.
-      destruct* H3; destruct_conjs.
+      admit.
+                
+    - unfold match_step.
       admit.
 
-    - unfold match_step.
-      intros c' Hin.
-      specializes H4 Hin.
-      destruct_conjs.
-      do 2 econstructor; splits*.
-      admit.
+    - admit.
+
+    - admit.
   Qed.
   
   Remark type_pres':
@@ -560,36 +640,40 @@ Section PRESERVATION.
         forall c,
           In c prog ->
           forall (WF: well_formed_stmt c S1 s)
-            e1 le1 m1 
-            (MS: match_states_bigbig c S1 (e1, le1, m1)),
+            (* e1 *) le1 m1 
+            (MS: match_states_bigbig c S1 ((* e1, *) le1, m1)),
           exists le2 m2 t,
-            exec_stmt tge (Clight.function_entry2 tge) e1 le1 m1 (translate_stmt c.(c_name) s)
+            exec_stmt tge (Clight.function_entry2 tge) Clight.empty_env le1 m1 (translate_stmt c.(c_name) s)
                        t le2 m2 ClightBigstep.Out_normal
-            /\ match_states_bigbig c S2 (e1, le2, m2))
+            /\ match_states_bigbig c S2 ((* e1, *) le2, m2))
     /\ (forall p me clsid vs me' rv,
           stmt_step_eval p me clsid vs me' rv ->
           sub_prog p prog ->
           (* p = prog -> *)
-          forall c S o c' prog' m loc_f f vptr e le,
+          forall c S o c' prog' m loc_f f loc_struct ofs (* e *) le,
             (* In c prog -> *)
             In c' prog ->
             well_formed_stmt c' (me, adds (Nelist.map_fst c'.(c_input)) vs v_empty) c'.(c_step) ->
-            match_states_bigbig c S (e, le, m) ->
+            match_states_bigbig c S ((* e, *) le, m) ->
             Globalenvs.Genv.find_symbol tge.(Clight.genv_genv) (step_id clsid) = Some loc_f ->
             Globalenvs.Genv.find_funct_ptr tge.(Clight.genv_genv) loc_f = Some (Ctypes.Internal f) ->
             find_inst o S me ->
             find_class clsid prog = Some (c', prog') ->
             List.length f.(Clight.fn_params) = 1 + Nelist.length vs ->
-            Clight.eval_expr tge e le m (ptr_obj (Some c.(c_name)) clsid o) vptr ->
+            Clight.eval_expr tge Clight.empty_env le m (ptr_obj (Some c.(c_name)) clsid o) (Values.Vptr loc_struct ofs) ->
+            valid_val rv f.(Clight.fn_return) ->
+            Clight.fn_return f <> Ctypes.Tvoid ->
+            (* Clight.eval_expr tge e le m (Clight.Etempvar (fst (c_output c')) (snd (c_output c'))) rv ->  *)
             exists m' t,
-              eval_funcall tge (Clight.function_entry2 tge) m (Ctypes.Internal f) (vptr :: nelist2list vs) t m' rv
-              /\ match_states_bigbig c (update_inst o S me') (e, le, m')
+              eval_funcall tge (Clight.function_entry2 tge) m (Ctypes.Internal f)
+                           ((Values.Vptr loc_struct ofs) :: nelist2list vs) t m' rv
+              /\ match_states_bigbig c (update_inst o S me') ((* e,  *)le, m')
         ).
   Proof.
     clear TRANSL.
     apply stmt_eval_step_ind;
       [| |introv ? ? ? ? Hifte|introv ? HS1 ? HS2|introv ? Evs ? Hrec_eval|
-       |(introv Hfind ? ? Hrec_exec; intros ** MS Hget_loc_f Hget_f ? Hfind' Hlengths ?)];
+       |(introv Hfind ? ? Hrec_exec; intros ** MS Hget_loc_f Hget_f ? Hfind' Hlengths ? ? ?)];
       intros;
       try inverts WF as; [|introv Hin| | |introv ? Hin Hfind Wfs ? Valids Types| |]; intros;
       inverts MS as Hvars Hself Hstep.
@@ -619,21 +703,20 @@ Section PRESERVATION.
           
     (* Comp s1 s2 : "s1; s2" *)
     - app_stmt_eval_det'.
-      edestruct HS1 with (e1:=e1); destruct_conjs; eauto.
+      edestruct HS1 (* with (e1:=e1) *); destruct_conjs; eauto.
       edestruct HS2; destruct_conjs; eauto.
       do 3 econstructor; split*.
       apply* exec_Sseq_1.
 
     (* Step_ap y ty clsid o [e1; ... ;en] : "y = clsid_step(&(self->o), e1, ..., en)" *)
     - app_exps_eval_det.
-
-      (* app_find_inst_det. *)
-      (* app_stmt_step_eval_det. *)
+      app_find_inst_det.
+      app_stmt_step_eval_det'.
       
       (* get the Clight corresponding function *)
       forwards* Hin': find_class_In Hfind.
       pose proof Hstep as Hstep'.
-      edestruct Hstep' as (loc_f & f & ? & ? & ? & Htype_fun & ? & ? & ? & ? & Hlengths & ?); eauto.
+      edestruct Hstep' as (loc_f & f & ? & ? & Htype_fun & ? & ? & ? & ? & Hlengths & ?); eauto.
       rewrite <-type_pres' with (c:=c) (es:=es) in Htype_fun; auto.
       forwards Eq: find_class_name Hfind.
       rewrite Eq in *; clear Eq.
@@ -645,23 +728,27 @@ Section PRESERVATION.
       specializes Hobj Hin; destruct Hobj as (delta).
 
       (* recursive funcall evaluation *)
-      app_find_inst_det.
-      edestruct Hrec_eval with (c:=c) (e:=e1) (m:=m1) (le:=le1); destruct_conjs; eauto.
+      edestruct Hrec_eval with (c:=c) (* (e:=e1) *) (m:=m1) (le:=le1); destruct_conjs; eauto.
       + rewrite <-ne_Forall2_lengths with (1:=Evs).
         rewrite Hlengths; simpl; f_equal. rewrite <-nelist2list_length.
         symmetry; apply* ne_Forall2_lengths.        
       + apply Clight.eval_Eaddrof; apply* evall_self_field.
-      + do 3 econstructor; split.
-        *{ eapply exec_Scall; eauto.
+      + inverts Htype_fun as ? Hret.
+        rewrite* Hret.
+      + inverts Htype_fun as ? Hret.
+        rewrite* Hret.
+      + do 3 econstructor; split*.
+        *{ apply* exec_Scall.
            - simpl; eauto.
            - eapply Clight.eval_Elvalue.
              + apply* Clight.eval_Evar_global.
+               apply Maps.PTree.gempty.
              + apply* Clight.deref_loc_reference.
            - econstructor.
              + eapply Clight.eval_Eaddrof.
                apply* evall_self_field.
              + eapply sem_cast_same.
-               unfold valid_val; splits~.
+               unfold valid_val; splits*.
                * discriminate.
                * simpl; trivial.
              + apply* exprs_eval_simu.
@@ -674,33 +761,40 @@ Section PRESERVATION.
       eapply exec_Sskip.
 
     (* funcall *)
-    - (* get the Clight function entry state *)
-      forwards* Hfind'': find_class_sub_same Hfind UNIQUE.
+    - forwards* Hfind'': find_class_sub_same Hfind UNIQUE.
       rewrite Hfind' in Hfind''; inverts Hfind''.
-      
-      (* rewrite Hfind in Hfind'; inverts Hfind'. *)
-      destruct Hstep with (c:=cls) as (loc_f' & f' & Hget_loc_f' & ? & Hget_f' & ? & ? & ? & ? & Htr & ?);
+      destruct Hstep with (c:=cls)
+        as (loc_f' & f' & Hget_loc_f' & Hget_f' & Htype_fun & Hvars_nil & ? & ? & Htr & ?);
         destruct_conjs; eauto.
       forwards Eq: find_class_name Hfind.
       rewrite Eq in Hget_loc_f'; clear Eq.
       rewrite Hget_loc_f' in Hget_loc_f; inverts Hget_loc_f.
       rewrite Hget_f' in Hget_f; inverts Hget_f.
 
-      assert (length f.(Clight.fn_params) = length (vptr :: nelist2list vs))
+      assert (length f.(Clight.fn_params) = length ((Values.Vptr loc_struct ofs) :: nelist2list vs))
         by (rewrite Hlengths; simpl; f_equal; rewrite Nelist.nelist2list_length; auto).
 
-      forwards* (m_fun & e_fun & le_fun & ? & ? & ?): (compat_funcall_pres cls m).
-      + skip.
-      + forwards* Hsub: find_class_sub.
-        subst env.
-        edestruct Hrec_exec with (e1:=e_fun) (le1:=le_fun) (m1:=m_fun); eauto.
-        destruct_conjs.
+      forwards* ((* m_fun & e_fun &  *)le_fun & ? & ?): (compat_funcall_pres cls m).
+      forwards* Hsub: find_class_sub.
+      subst env.
+      edestruct Hrec_exec with (* (e1:=e_fun) *) (le1:=le_fun) (* (m1:=m_fun) *) as (le2 & m2 & ? & ? & MS); eauto.
+      destruct_conjs.
         
-        do 2 econstructor; split.
-        apply* eval_funcall_internal.
-        * constructor*.
-        * rewrite* Htr.
-        * admit.
-        * skip.
-        * skip.
+      do 2 econstructor; split.
+      apply* eval_funcall_internal.
+      + constructor*; rewrite Hvars_nil; simpl; constructor.
+      + rewrite* Htr.
+        apply* exec_Sseq_1.
+        apply* exec_Sreturn_some.
+        apply* Clight.eval_Etempvar.
+        inverts MS as Hvars'.
+        apply* Hvars'.
+        rewrite <-surjective_pairing.
+        eapply in_eq.
+      + simpl; split*.
+        inverts Htype_fun.
+        apply* sem_cast_same.
+      + simpl. eauto.       
+      + constructor*.
+        admit.
   Qed.
